Update Introduction

tutorial/Introduction.v
@@ -1,13 +1,22 @@
+(** * Introduction to interaction trees *)
+
+(** This file gives and example of defining recursive functions
+    using ITrees. It demonstrates
+    - [rec]
+    - equational reasoning using [≈] ([\approx])
+*)
+
 (* begin hide *)
 Set Implicit Arguments.
 Set Contextual Implicit.
 
 From Coq Require Import
-     Nat
+     Arith
      Setoid
      RelationClasses
      Program
-     Morphisms.
+     Morphisms
+     Lia.
 
 From ExtLib Require Import
      Monad.
@@ -15,68 +24,16 @@ From ExtLib Require Import
 From ITree Require Import
      Simple.
 
+Import ITreeNotations.
 Import MonadNotation.
 Open Scope monad_scope.
 (* end hide *)
 
+(** In this file, we won't use external effects, so we will use this
+    empty effect type [void1]. *)
 Definition E := void1.
 
-(** * Factorial Example *)
-
-(** * Factorial *)
-
-(** This file gives and example of defining a recursive version of the "factorial" 
-    function using ITrees. It demonstrates
-       - [rec]
-       - equational reasoning using ≈
-*)
-
-(** The generic [rec] interface of the library's [Interp] module can be used to
-    define a single recursive function.  The more general [mrec] (from which [rec] is defined)
-    allows multiple, mutually recursive definitions.
-
-    To use [rec], we instantiate the generic "recursive" call event [callE] at the 
-    desired type.  In this case, since, [factorial : nat -> nat], we use [callE nat nat].
-*)
-
-(** [factC] is an event representing the recursive call.  Since in general, the 
-    function might have other effects of type [E], the resulting itree has 
-    type [(callE nat nat +' E)].  [factC] simply injects the argument [n] into the 
-    event.
- *)
-
-(** We write the body of the function monadically, using events rather than recursive calls. *)
-Definition fact_body (x : nat) : itree (callE nat nat +' E) nat :=
-  match x with
-  | 0 => Ret 1
-  | S m => y <- call m ;; Ret (x * y)
-  end.
-
-(** The factorial function itself is defined as an itree by 'tying the knot' using [rec]. 
-
-    (Aside: Note that [factorial] is actually a [KTree] of type [ktree nat nat].)
-*)
-Definition factorial (n : nat) : itree E nat :=
-  rec fact_body n.
-
-Example fact_5 : exists y, factorial 5 ≈ Ret y.
-Proof.
-  eexists.
-  tau_steps.
-  reflexivity.
-Qed.
-
-(** An equivalent definition with a [rec-fix] notation looking like [fix].
- *)
-Definition factorial' : nat -> itree E nat :=
-  rec-fix fact x :=
-    match x with
-    | 0 => Ret 1
-    | S m => y <- fact m ;; Ret (x * y)
-    end.
-
-Lemma factorial_same : factorial = factorial'.
-Proof. reflexivity. Qed.
+(** ** Factorial *)
 
 (** This is the Coq specification -- the usual mathematical definition. *)
 Fixpoint factorial_spec (n : nat) : nat :=
@@ -85,103 +42,249 @@ Fixpoint factorial_spec (n : nat) : nat :=
   | S m => n * factorial_spec m
   end.
 
-(** We can prove that the ITrees version [factorial] is "equivalent" to the
-    [factorial_spec] version.  The proof goes by induction on n and uses only
-    rewriting -- no coinduction necessary. Here, we step through each step of
-    rewriting to illustrate the use of the equational theory, which is mostly
-    applications of the monad laws and the properties of [rec], seen as an 
-    instance of [mrec]. 
+(** The generic [rec] interface of the library's [Interp] module can
+    be used to define a single recursive function.  The more general
+    [mrec] (from which [rec] is defined) allows multiple, mutually
+    recursive definitions.
+
+    The argument of [rec] is an interaction tree with an effect
+    [callE A B] to represent "recursive calls", with input [A]
+    and output [B]. The function [call : A -> itree _ B] can be used
+    to make such calls.
+
+    In this case, since [factorial : nat -> nat], we use
+    [callE nat nat].
+ *)
+Definition fact_body (x : nat) : itree (callE nat nat +' E) nat :=
+  match x with
+  | 0 => Ret 1
+  | S m =>
+    y <- call m ;;  (* Recursively compute [y := m!] *)
+    Ret (x * y)
+  end.
+
+(** The factorial function itself is defined as an itree by "tying
+    the knot" using [rec].
+ *)
+Definition factorial (n : nat) : itree E nat :=
+  rec fact_body n.
+
+(** Contrary to definitions by [Fixpoint], there are no restrictions
+    on the arguments of recursive calls: [rec] may thus produce
+    diverging computations, and Coq will not naively reduce
+    [factorial 5].
+
+    Of course, we can force the computation with fuel, e.g.,
+    using [burn]...
+ *)
+Compute (burn 100 (factorial 5)).
+
+(** ... or with tactics, such as [tau_steps], which removes
+    all taus from the left-hand side of an [≈] equation. *)
+Example fact_5 : factorial 5 ≈ Ret 120.
+Proof.
+  tau_steps.
+  reflexivity.
+Qed.
+
+(** An equivalent definition with a [rec-fix] notation looking like
+    [fix], where the recursive call can be given a more specific name.
+ *)
+Definition factorial' : nat -> itree E nat :=
+  rec-fix fact x :=
+    match x with
+    | 0 => Ret 1
+    | S m => y <- fact m ;; Ret (x * y)
+    end.
+
+(** These two definitions are definitionally equal. *)
+Lemma factorial_same : factorial = factorial'.
+Proof. reflexivity. Qed.
+
+(** We can prove that the ITrees version [factorial] is "equivalent"
+    to the [factorial_spec] version.  The proof goes by induction on
+    [n] and uses only rewriting -- no coinduction necessary.
+
+    Here, we detail each step of rewriting to illustrate the use of
+    the equational theory, which is mostly applications of the monad
+    laws and the properties of [rec].
 
     In this proof, we do all of the rewriting steps explicitly.
-*)
-Lemma factorial_correct : forall n, factorial n ≈ Ret (factorial_spec n).
+ *)
+Lemma factorial_correct : forall n,
+    factorial n ≈ Ret (factorial_spec n).
 Proof.
   intros n.
-  induction n; intros; subst.
-  - unfold factorial. rewrite rec_as_interp. simpl. rewrite interp_ret. reflexivity.
-  - unfold factorial. rewrite rec_as_interp. simpl.
+  unfold factorial.
+  induction n as [ | n' IH ].
+  - (* n = 0 *)
+    rewrite rec_as_interp. simpl.
+    rewrite interp_ret.
+    reflexivity.
+  - (* n = S n' *)
+    rewrite rec_as_interp. simpl.
     rewrite interp_bind.
     rewrite interp_recursive_call.
-    rewrite IHn.
+    rewrite IH.                   (* Induction hypothesis *)
     rewrite bind_ret.
     rewrite interp_ret.
     reflexivity.
 Qed.
 
-(** * Fibonacci *)
+(** The tactics [tau_steps] and [autorewrite with itree] offer
+    a little automation to simplify monadic expressions. *)
+Lemma factorial_correct' : forall n,
+    factorial n ≈ Ret (factorial_spec n).
+Proof.
+  intros n.
+  unfold factorial.
+  induction n as [ | n' IH ].
+  - (* n = 0 *)
+    tau_steps. (* Just compute away. *)
+    reflexivity.
+  - (* n = S n' *)
+    rewrite rec_as_interp.
+    unfold fact_body at 2.
+    autorewrite with itree.
+    rewrite IH.             (* Induction hypothesis *)
+    autorewrite with itree.
+    reflexivity.
+Qed.
+
+(** ** Fibonacci *)
 
 (** Exercise *)
-(** Carry out the analogous proof of correctness for the Fibonacci function, whose
-    naturally recursive coq definition is given below. *)
+(** Carry out the analogous proof of correctness for the Fibonacci
+    function, whose naturally recursive coq definition is given below.
+ *)
 
 Fixpoint fib_spec (n : nat) : nat :=
   match n with
-  | 0 => 1
-  | S m =>
-    match m with
+  | 0 => 0
+  | S n' =>
+    match n' with
     | 0 => 1
-    | S k => fib_spec m + fib_spec k
+    | S n'' => fib_spec n'' + fib_spec n'
     end
   end.
 
-(** We write the body of the fib monadically, using events rather than recursive calls. *)
 Definition fib_body : nat -> itree (callE nat nat +' E) nat :=
 (* SOLN *)  
-  fun x => match x with
-        | 0 => Ret 1
-        | S m =>
-          match m with
-          | 0 => Ret 1
-          | S k => y1 <- call m ;;
-                  y2 <- call k ;;
-                  Ret (y1 + y2)
-          end
-        end.
-(* STUBWITH Ret 0 *)
-
-Require Import Omega.
+  fun n =>
+    match n with
+    | 0 => Ret 0
+    | S n' =>
+      match n' with
+      | 0 => Ret 1
+      | S n'' =>
+        y1 <- call n'' ;;
+        y2 <- call n' ;;
+        Ret (y1 + y2)
+      end
+    end.
+(* STUBWITH (fun n => Ret 0) *)
 
 Definition fib n : itree E nat :=
   rec fib_body n.
 
-(** Since fib uses two recursive calls, we need to strengthen the induction hypothesis.  One way
-   to do that is to prove the property for all [m <= n]. *)
-(* SAZ: is this a good example? The stronger induction hypothesis is kind of orthogonal to the 
-   point we're trying to make. *)
+(** Since fib uses two recursive calls, we need to strengthen the
+    induction hypothesis.  One way to do that is to prove the
+    property for all [m <= n].
+
+    You may find the following two lemmas useful at the start
+    of each case.
+[[
+Nat.le_0_r : forall n : nat, n <= 0 <-> n = 0
+Nat.le_succ_r : forall n m : nat, n <= S m <-> n <= m \/ n = S m
+]]
+ *)
+
 Lemma fib_correct : forall n m, m <= n ->
     fib m ≈ Ret (fib_spec m).
 Proof.
 (* SOLN *)  
   intros n.
-  induction n; intros; subst.
-  - apply Le.le_n_0_eq in H. subst. 
-    unfold fib.  rewrite rec_as_interp. simpl. rewrite interp_ret.  reflexivity.
-  - induction m; intros; subst.
-    + unfold fib. rewrite rec_as_interp. simpl. rewrite interp_ret. reflexivity.
-    + unfold fib.
-      rewrite rec_as_interp. simpl.
-      destruct m.
+  unfold fib.
+  induction n as [ | n' IH ]; intros.
+  - (* n = 0 *)
+    apply Nat.le_0_r in H. subst m.
+    unfold fib.
+    rewrite rec_as_interp. simpl.
+    rewrite interp_ret.
+    (* alternatively, [tau_steps], or [autorewrite with itree] *)
+    reflexivity.
+  - (* n = S n' *)
+    apply Nat.le_succ_r in H.
+    destruct H.
+    + apply IH; auto.
+    + rewrite rec_as_interp.
+      subst m. simpl.
+      destruct n' as [ | n'' ].
       * rewrite interp_ret. reflexivity.
-      * rewrite interp_bind. rewrite interp_recursive_call. rewrite IHm.
-        rewrite bind_ret. rewrite interp_bind. rewrite interp_recursive_call.
-        unfold fib in IHn. rewrite IHn. rewrite bind_ret.
-        rewrite interp_ret. reflexivity.
-        omega. omega. 
+      * autorewrite with itree.
+        rewrite IH. 2: lia.
+        autorewrite with itree.
+        rewrite IH. 2: lia.
+        autorewrite with itree.
+        reflexivity.
 Qed.
 (* STUBWITH Admitted. *)
 
-(** Logarithm *)
+(** ** Logarithm *)
+
+(** An example of a function which is not structurally recursive:
+    logarithm in base [b].
+ *)
 
 Definition log_ (b : nat) : nat -> itree E nat :=
   rec-fix log_b n :=
-    if n =? O then
+    if n <=? 1 then
       Ret O
     else
       y <- log_b (n / b) ;; Ret (S y).
 
-Example log_2_100 : exists y, log_ 2 100 ≈ Ret y.
+Example log_2_64 : log_ 2 (2 ^ 6) ≈ Ret 6.
 Proof.
-  eexists.
   tau_steps.
   reflexivity.
+Qed.
+
+(** We can prove that [log_ b (b ^ y) ≈ Ret y] when [1 < b]. *)
+
+(** These lemmas take care of the boring arithmetic. *)
+Lemma log_correct_helper :
+  forall b y, 1 < b ->
+              (b * b ^ y <=? 1) = false.
+Proof.
+  intros.
+  apply Nat.leb_gt.
+  apply Nat.lt_1_mul_pos; auto.
+  apply neq_0_lt. intro.
+  apply (Nat.pow_nonzero b y); lia.
+Qed.
+
+Lemma log_correct_helper2 :
+  forall b y, 1 < b ->
+              (b * b ^ y / b) = (b ^ y).
+Proof.
+  intros; rewrite Nat.mul_comm, Nat.div_mul; lia.
+Qed.
+
+Lemma log_correct : forall b y, 1 < b -> log_ b (b ^ y) ≈ Ret y.
+Proof.
+  intros b y H.
+  unfold log_, rec_fix.
+  induction y.
+  - rewrite rec_as_interp; cbn.
+    autorewrite with itree.
+    reflexivity.
+  - rewrite rec_as_interp; cbn.
+    (* (b * b ^ y <=? 1) = false *)
+    rewrite log_correct_helper by auto.
+    autorewrite with itree.
+    (* (b * b ^ y / b) = (b ^ y)*)
+    rewrite log_correct_helper2 by auto.
+    rewrite IHy.
+    autorewrite with itree.
+    reflexivity.
 Qed.
